src/Helpers/List.v
@@ -1,0 +1,49 @@
+From stdpp Require Import list.
+From Coq Require Import ssreflect.
+
+Section list.
+  Context (A:Type).
+  Notation list := (list A).
+  Implicit Types (l:list).
+
+  Definition Forall_idx (P: nat -> A -> Prop) (start:nat) (l: list): Prop :=
+    Forall2 P (seq start (length l)) l.
+
+  Lemma drop_seq n len m :
+    drop m (seq n len) = seq (n + m) (len - m).
+  Proof.
+    revert n m.
+    induction len; simpl; intros.
+    - rewrite drop_nil //.
+    - destruct m; simpl.
+      + replace (n + 0)%nat with n by lia; auto.
+      + rewrite IHlen.
+        f_equal; lia.
+  Qed.
+
+  Theorem Forall_idx_drop (P: nat -> A -> Prop) l (start n: nat) :
+    Forall_idx P start l ->
+    Forall_idx P (start + n) (drop n l).
+  Proof.
+    rewrite /Forall_idx.
+    intros.
+    rewrite drop_length -drop_seq.
+    apply Forall2_drop; auto.
+  Qed.
+
+  Theorem Forall_idx_impl (P1 P2: nat -> A -> Prop) l (start n: nat) :
+    Forall_idx P1 start l ->
+    (forall i x, l !! i = Some x ->
+            P1 (start + i)%nat x ->
+            P2 (start + i)%nat x) ->
+    Forall_idx P2 start l.
+  Proof.
+    rewrite /Forall_idx.
+    intros.
+    apply Forall2_same_length_lookup.
+    eapply Forall2_same_length_lookup in H.
+    intuition idtac.
+    pose proof (lookup_seq_inv _ _ _ _ H); intuition subst.
+    apply H0; eauto.
+  Qed.
+End list.
